Without panics

BellmanFord/BellmanFord.lean
@@ -1,6 +1,68 @@
-import Graph.Dijkstra
+import Graph.Path 
 
 namespace Graph
+
+structure Edge (β : Type) where
+  target : Nat
+  weight : β
+
+structure Vertex (α : Type) (β : Type) where
+  payload : α
+  adjacencyList : List (Edge β) := []
+
+instance [Inhabited α] : Inhabited (Vertex α β) := ⟨ { payload := default } ⟩
+
+end Graph
+
+structure Graph (α : Type) (β : Type) where
+  vertices : List (Graph.Vertex α β) := []
+
+namespace Graph
+
+variable {α : Type} [Inhabited α] {β : Type}
+
+/-- Empty graph, α is the vertex payload type, β is edge weight type --/
+def empty : Graph α β := ⟨[]⟩
+
+/-- Total edge count in the graph. -/
+def edgeCount (g : Graph α β) : Nat := g.vertices.foldr (λ vertex count => vertex.adjacencyList.length + count) 0
+
+def vertexCount (g : Graph α β) : Nat := g.vertices.length
+
+def getAllVertexIDs (g : Graph α β) : List Nat := Id.run do
+  let mut arr := mkArray g.vertexCount 0
+  for i in [0:g.vertexCount] do arr := arr.set! i i
+  arr.toList
+
+def makeGraphFromArray (a : List α) : Graph α β := ⟨
+  a.map (λ element => { payload := element } )
+⟩
+
+def addVertex (g : Graph α β) (payload : α) : (Graph α β) × Nat :=
+  let res := { g with vertices := g.vertices.append [{ payload := payload }] }
+  let id : Nat := res.vertexCount - 1
+  (res, id)
+
+def addEdgeByID (g : Graph α β) (source : Nat) (target : Nat) (weight : β) : Graph α β := {
+  g with vertices := (g.vertices.toArray.modify source (λ vertex => { vertex with adjacencyList := (vertex.adjacencyList.toArray.push {target := target, weight := weight}).toList })).toList
+}
+
+namespace Vertex
+
+private def toString [ToString α] [ToString β] (v : Vertex α β) : String := "\nVertex payload: " ++ ToString.toString v.payload ++ ", edges:\n" ++ v.adjacencyList.foldr foldEdges "" ++ "\n"
+  where foldEdges (e : Edge β) (s : String) : String :=
+    s ++ "   target: " ++ (ToString.toString e.target) ++ ", weight: " ++ (ToString.toString e.weight) ++ "\n"
+
+instance [ToString α] [ToString β] : ToString (Vertex α β) where toString := toString
+
+end Vertex
+
+instance [ToString α] [ToString β] : ToString (Graph α β) where toString :=
+  (λ g => toString (g.getAllVertexIDs.zip g.vertices))
+
+end Graph
+
+/---End of Graph Libray---/
 
 /- Approach for Bellman-Ford
 
@@ -34,6 +96,8 @@ If there are no negative cycles detected, we return Distance and Predecessor arr
 
 -/
 
+namespace Graph
+
 /-!
 ## Bellman-Ford Algorithm
 
@@ -63,7 +127,7 @@ instance : Inhabited BFVertex := ⟨ { predecessor := default } ⟩
 ----------BFShortestPathTree----------
 
 structure BFShortestPathTree where
-  BFVertices : Array BFVertex
+  BFVertices : List BFVertex
 
 namespace BFShortestPathTree
 
@@ -87,7 +151,7 @@ private def pathToVertexAux (t : BFShortestPathTree) (id : Nat) (pathSoFar : Pat
 /--Returns the shortest path from the tree root to the specified vertex--/
 def pathToVertex (t : BFShortestPathTree) (id : Nat) : Option (Path Int true) := match t.BFVertices[id]!.distance with
   | none => none
-  | some _ => some (pathToVertexAux t id Path.empty t.BFVertices.size)
+  | some _ => some (pathToVertexAux t id Path.empty t.BFVertices.length)
 
 end BFShortestPathTree
 
@@ -95,34 +159,38 @@ end BFShortestPathTree
 
 ----------BFAlgo----------
 
+def BF_rec  (edge : Edge Int) (combined : Nat × List BFVertex): Nat × List BFVertex  :=
+    let (vertex,BFVertices) := combined
+    if  h : edge.target < BFVertices.length then
+      let tentativeDistance : Option Int := match BFVertices[vertex]!.distance with -- creating new distance for edge.target. treat "none" as infinity.
+        | some x => x + edge.weight
+        | none => none
+      let newBFVertex : BFVertex := {predecessor := vertex, distance := tentativeDistance, edgeWeightToPredecessor := edge.weight} -- new BFVertex to represent edge.target
+      let BFVertices_final := match BFVertices[edge.target].distance with
+        | some x => match newBFVertex.distance with -- again, treat none as infinity here, and the logic should be clear. if previous distance is larger than new distance, replace the BFVertex. Otherwise let it be.
+                    | some y => if y < x then BFVertices.set edge.target newBFVertex else BFVertices
+                    | none => BFVertices
+        | none => BFVertices.set edge.target newBFVertex    
+      (vertex, BFVertices_final)
+    else combined
+      
+
 /--BFAux2 takes the graph, a vertex and the BFVertices array and iterates over the edges from the vertex, updating
 distances and predecessors in BFVertices as described in the algorithm above--/
-private def BFAux2 (g : Graph α Int) (vertex : Nat) (BFVerticesTemp : Array BFVertex) : Array BFVertex := Id.run do
-  let mut BFVertices : Array BFVertex := BFVerticesTemp
-  for edge in g.vertices[vertex]!.adjacencyList do -- for each edge in adj list of vertex
-    let tentativeDistance : Option Int := match BFVertices[vertex]!.distance with -- creating new distance for edge.target. treat "none" as infinity.
-      | some x => x + edge.weight
-      | none => none
-    let newBFVertex : BFVertex := {predecessor := vertex, distance := tentativeDistance, edgeWeightToPredecessor := edge.weight} -- new BFVertex to represent edge.target
-    BFVertices := match BFVertices[edge.target]!.distance with
-      | some x => match newBFVertex.distance with -- again, treat none as infinity here, and the logic should be clear. if previous distance is larger than new distance, replace the BFVertex. Otherwise let it be.
-                  | some y => if y < x then BFVertices.set! edge.target newBFVertex else BFVertices
-                  | none => BFVertices
-      | none => BFVertices.set! edge.target newBFVertex
-  return BFVertices
+def BFAux2 (g : Graph α Int) (vertex : Nat) (BFVertices : List BFVertex) : List BFVertex :=
+    if h:vertex < g.vertices.length then
+      (g.vertices[vertex].adjacencyList.foldr BF_rec (vertex,BFVertices)).2
+    else BFVertices
 
 /--BFAux recurses over itself n times, where n = g.vertexCount - 1. Every iteration, it goes over every edge in the graph and updates distance and predecessors as described in the algorithm--/
-private def BFAux (g : Graph α Int) (BFVerticesTemp : Array BFVertex) : Nat -> Array BFVertex
-  | 0 => BFVerticesTemp
-  | n + 1 => Id.run do --for recursion
-    let mut BFVertices : Array BFVertex := BFVerticesTemp
-    for vertex in g.getAllVertexIDs do -- for each vertex in g, we update distances and predecessors for each edge in g.vertices[vertex].adjacencyList.
-      BFVertices := BFAux2 g vertex BFVertices
-    BFAux g BFVertices n --for recursion.
+def BFAux (g : Graph α Int) (BFVertices : List BFVertex) : Nat -> List BFVertex
+  | 0 => BFVertices
+  | n + 1 =>  --for recursion 
+    BFAux g (g.getAllVertexIDs.foldl (λ BFVertices vertex => BFAux2 g vertex BFVertices) BFVertices) n --for recursion.
 
 ---The negative cycle detection---
 
-private def negative_cycle_detection_edge (i : Nat) (edge : Edge Int) (w : Array BFVertex) : Bool :=
+private def negative_cycle_detection_edge (i : Nat) (edge : Edge Int) (w : List BFVertex) : Bool :=
     match w[i]!.distance with
     | none => true
     | some u => 
@@ -134,31 +202,30 @@ private def negative_cycle_detection_edge (i : Nat) (edge : Edge Int) (w : Array
             else
               true
 
-private def negative_cycle_detection (g : Graph α Int) (w : Array BFVertex) (nncycle : Bool) : Nat → Bool 
+private def negative_cycle_detection (g : Graph α Int) (w : List BFVertex) (nncycle : Bool) : Nat → Bool 
     | 0 => nncycle
-    | n + 1 => Id.run do
-        let mut no_neg_cycle : Bool := true
-        for edge in g.vertices[n]!.adjacencyList do
-            no_neg_cycle :=
-              match (negative_cycle_detection_edge (n) edge w) with
-              | true => no_neg_cycle
-              | false => false
-        negative_cycle_detection g w (nncycle ∧ no_neg_cycle) n
+    | n + 1 => 
+        if h : n < g.vertices.length then 
+          negative_cycle_detection g w (g.vertices[n].adjacencyList.foldl (λ nncycle edge =>  
+                                                                             match (negative_cycle_detection_edge (n) edge w) with
+                                                                             | true => nncycle
+                                                                             | false => false) nncycle) n
+        else false
 
 ---End of negative cycle detection algorithm---
 
-private def BFAuxBase (g : Graph α Int) (source : Nat) : Array (BFVertex) :=
-  let BFVerticesInitial : Array (BFVertex) := mkArray g.vertexCount {predecessor := source} -- predecessor is only a placeholder here, it has no significance and will be replaced or not used
-  if h : source < BFVerticesInitial.size then
-    let BFVertices := BFVerticesInitial.set ⟨source, h⟩ {predecessor := source, distance := some 0}
-    let BFVerticesUpdated : Array (BFVertex) := BFAux g BFVertices (g.vertexCount - 1)
+private def BFAuxBase (g : Graph α Int) (source : Nat) : List (BFVertex) :=
+  let BFVerticesInitial : List (BFVertex) := (mkArray g.vertexCount {predecessor := source}).toList -- predecessor is only a placeholder here, it has no significance and will be replaced or not used
+  if h : source < BFVerticesInitial.length then
+    let BFVertices := BFVerticesInitial.set source {predecessor := source, distance := some 0}
+    let BFVerticesUpdated : List (BFVertex) := BFAux g BFVertices (g.vertexCount - 1)
     match (negative_cycle_detection g BFVerticesUpdated true g.vertexCount) with
     | true => BFVerticesUpdated
     | false => panic! "The Graph has negative cycle"
   else
       panic! "source out of bounds"
 
-def BellmanFord (g : Graph α Int) (source : Nat) : Array BFVertex := BFAuxBase g source -- call this function to turn BF Algorithm on a given graph g at vertex source.
+def BellmanFord (g : Graph α Int) (source : Nat) : List BFVertex := BFAuxBase g source -- call this function to turn BF Algorithm on a given graph g at vertex source.
 
 def BFShortestPath (g : Graph α Int) (source : Nat) (target : Nat) : Option (Path Int true) :=
   let BFshortestPathTree : BFShortestPathTree := ⟨ (BFAuxBase g source ) ⟩
@@ -174,16 +241,35 @@ def BFShortestPath (g : Graph α Int) (source : Nat) (target : Nat) : Option (Pa
   we only need one iteration-/
 
 /-It takes a graph, weight array and a edge as input and outputs the updated graph and updated weight array-/
-def BF_dynamic_edgeAdd (g : Graph α Int) (w: Array BFVertex) (edge : Nat × Nat × Int) : Graph α Int × Array BFVertex :=
+def BF_dynamic_edgeAdd (g : Graph α Int) (w: List BFVertex) (edge : Nat × Nat × Int) : Graph α Int × List BFVertex :=
     let g_updated := addEdgeByID g edge.1 edge.2.1 edge.2.2
     ⟨ g_updated, (BFAux g_updated w) 1 ⟩
 
 /-It takes a a graph, weight array and a vertex as input and outputs the updated graph and updated weight array-/
-def BF_dynamic_vertex_addition (g : Graph Nat Int) (w: Array BFVertex) (vertex : Vertex Nat Nat) : Graph Nat Int × Array BFVertex := 
+def BF_dynamic_vertex_addition (g : Graph Nat Int) (w: List BFVertex) (vertex : Vertex Nat Nat) : Graph Nat Int × List BFVertex := 
     let g_updated := (addVertex g vertex.payload).fst  
     ⟨ g_updated, (BFAux g_updated w) 1⟩
 
 
 ----------End of Dynamic allocation----------
 
-end Graph
+def g_array : List Nat := [1,2,3,4,5]
+
+def g : Graph Nat Int := makeGraphFromArray g_array
+
+/-It takes a graph g and a array of edges (of form ((u,v),weight of edge u to v)) as input and outputs a graph with these array of edges-/
+private def adding_edges_by_arrays {α : Type} (g : Graph α Int) (as : List (List Nat × Int)) : Graph α Int := Id.run do
+    let mut ret : Graph α Int := g
+    for i in as do
+        ret := addEdgeByID ret (i.fst[0]!-1) (i.fst[1]!-1) i.snd 
+    ret
+def g_final := adding_edges_by_arrays g ([([1,2],5),([2,1],-2),([3,2],7),([4,3],9),([1,4],8),([1,3],-4),([5,1],6),([5,4],7),([3,5],2),([4,2],-3)])
+
+#eval g_final
+
+def BF_weight_array := BellmanFord g_final 4
+
+def BF_shortest_path := BFShortestPath g_final 1 2
+
+#eval BF_weight_array ---weight array
+#eval BF_shortest_path 
