lakefile.lean
@@ -9,6 +9,10 @@ lean_lib «BellmanFord» {
   -- add library configuration options here
 }
 
+lean_lib «Graph_lib» {
+  -- add library configuration options here
+}
+
 require mathlib from git
   "https://github.com/leanprover-community/mathlib4.git"@"master"
 
